The expression \( x^{2} + 7x - 60 \) is a quadratic
expression. We are being asked to factor it into the product of two
*binomials*. To see which of these choices is equivalent to the given
quadratic expression, we can use the distributive property to multiply
each of the choices. When multiplying two binomials as shown in each of
the answer choices, we can use FOIL (First, Outer, Inner, Last):

A.  (x+12)(x-5) = x^2^ – 5x + 12x -60 = x^2^ + 7x -60

B.  (x+10)(x-6) = x^2^ – 6x + 10x -60 = x^2^ + 4x -60

C.  (x+15)(x-4) = x^2^ – 4x + 15x -60 = x^2^ + 11x -60

D.  (x+20)(x-3) = x^2^ – 3x + 20x -60 = x^2^ + 17x -60

Choice A is the product that is equivalent to the given quadratic
expression.

You can review multiplying binomials using FOIL here:
<http://www.virtualnerd.com/pre-algebra/polynomials-nonlinear-functions/binomial-multiplication/foil-multiply-binomials/foil-method-example-problem>
