We are asked to find a value of x that satisfies both of
the equations

$$3x - 2y = 6$$

$$x + 2y = 10$$

Since we are asked to find the value of the variable *x*, we need to
find a way to eliminate the variable *y*. We can start with either
equation, so letâ€™s start with the second one (that way we do not have to
contend with the subtraction in front of the *y* that we see in the
first equation). From the second equation, we can subtract *x* from both
sides of the equation to get

$$2y = 10 - x$$

Normally when solving a system of two linear equations, we would want to
divide both sides by 2 so that we have *y* by itself. But, in this case,
there is a shortcut. Notice that the first equation has the expression
*2y* in it as well, so we can take our new expression for *2y* and
substitute it in place of the *2y* in the first equation, like this:

$$3x - 2y = 6$$

$$3x - (10 - x) = 6$$

Now we have an equation with only one variable, and we can solve for
*x*. The order of operations

$$3x - 10 + x = 6$$

(remember that two negatives make a positive: --x = +x). Combine 3x + x
= 4x:

$$4x - 10 = 6$$

Then add 10 to both sides

$$4x = 16$$

And divide by 4.

$$x = 4$$

You can review strategies for solving systems of equations here:
<http://www.virtualnerd.com/algebra-2/linear-systems/equations-solution-by-substitution.php>

Or a slightly more complicated example here:
<http://www.virtualnerd.com/algebra-1/systems-equations-inequalities/two-equations-two-variables-substitution.php>
