The first step in finding the product is to multiply the
two expressions:

$$4\sqrt{2} \times 2\sqrt{6} = 8\sqrt{12}$$

Since this is not one of the choices, it seems that we need to simplify
this expression. Notice that since 12 = 4 x 3,

$$\sqrt{12} = \ \sqrt{4} \times \sqrt{3} = 2\sqrt{3}$$

Substituting that into the original expression we get

$$4\sqrt{2} \times 2\sqrt{6} = 8\sqrt{12} = 8 \times 2\sqrt{3} = 16\sqrt{3}$$

Learn more about simplifying expressions with square roots here:
<https://www.mathsisfun.com/numbers/simplify-square-roots.html>
