There are several ways to solve this problem. The most
straightforward one is to recognize that the second equation defines a,
so we can substitute that expression ($\frac{1}{2}b - 6)\ $for a in the
first equation.

$$2\left( \frac{1}{2}b - 6 \right) + 3b = 12$$

Using the distributive property, we get

$$b - 12 + 3b = 12$$

$$4b - 12 = 12$$

$$4b = 24$$

$$b = 6$$

Once we get b=6, that value can be substituted back into either equation
to find the value of a. It will work with either equation, but letâ€™s try
it with the second equation:

$$a = \ \frac{1}{2}\left( 6 \right) - 6 = 3 - 6 = \  - 3$$

So, a = -3 and b = 6. You can check that this is the correct solution by
substituting those values for a and b into both of the equations.
