The given equation involves algebraic fractions, so the
first step is to simplify the denominators. Remember that we can
multiply both sides of the equation by the same expression, and the
equation will be equivalent. If we multiply both sides of the equation
by 3 (the denominator on the left side), we get:

$3\  \times \frac{x}{3} = \frac{8}{x + 2} \times 3\ $

Which is equivalent to

$x = \frac{24}{x + 2}\ $

That made the equation simpler by removing the fraction from the left
side of the equation, and we can do the same for the fraction on the
right side by multiplying both sides by *x+2*:

$(x + 2) \times x = \frac{24}{x + 2} \times (x + 2)\ $

The (x+2) terms on the right side of the equation cancel, resulting in

$x^{2} + 2x = 24\ $

Notice that this is the same result you would get if you
“cross-multiply”.

$x^{2} + 2x - 24 = 0\ $

This can be factored as

$$(x + 6)(x - 4) = 0$$

The only way that the product of two quantities can equal zero is if at
least one of them equals zero, so either x+6=0 or x-4=0. That leads to
the two solutions x=-6 or x=4.

To learn more about working with fractions in algebra, see

<http://www.themathpage.com/alg/algebraic-fractions.htm>

You can review *factoring a quadratic polynomial* here:
<http://www.mathsisfun.com/algebra/factoring-quadratics.html>
