We can simplify this expression by combining the numbers,
the x terms, and the y terms.

First, the numbers: \( \frac{24}{- 6} = \  - 4 \).

Then, the x's:

$$\frac{x^{6}}{x^{3}} = \frac{x \bullet x \bullet x \bullet x \bullet x \bullet x}{x \bullet x \bullet x} = x^{3}$$

And finally the y's:

$$\frac{y^{3}}{y} = \ \frac{y \bullet y \bullet y}{y} = y^{2}$$

Put those pieces together, and

$$\frac{24x^{6}y^{3}}{- 6x^{3}y} = - 4x^{3}y^{2}$$ 

which is choice (4). To
review algebraic expressions with exponents, see
<http://www.mathsisfun.com/algebra/exponent-laws.html>
